src/Bedrock/Proofs/LoadStoreList.v
@@ -1,0 +1,436 @@
+Require Import Coq.ZArith.ZArith.
+Require Import Coq.Strings.String.
+Require Import Coq.Lists.List.
+Require Import Coq.micromega.Lia.
+Require Import bedrock2.Array.
+Require Import bedrock2.Scalars.
+Require Import bedrock2.Syntax.
+Require Import bedrock2.ProgramLogic.
+Require Import bedrock2.Map.Separation.
+Require Import bedrock2.Map.SeparationLogic.
+Require Import bedrock2.WeakestPreconditionProperties.
+Require Import coqutil.Word.Interface coqutil.Word.Properties.
+Require Import coqutil.Map.Interface coqutil.Map.Properties.
+Require Import Crypto.Bedrock.Types.
+Require Import Crypto.Bedrock.Tactics.
+Require Import Crypto.Bedrock.Proofs.Dexprs.
+Require Import Crypto.Bedrock.Proofs.Flatten.
+Require Import Crypto.Bedrock.Proofs.Varnames.
+Require Import Crypto.Bedrock.Translation.Flatten.
+Require Import Crypto.Bedrock.Translation.LoadStoreList.
+Require Import Crypto.Language.API.
+Require Import Crypto.Util.ListUtil.
+Import ListNotations.
+
+Import API.Compilers.
+Import Types.Notations Types.Types.
+
+Section LoadStoreList.
+  Context {p : parameters} {p_ok : @ok p}.
+
+  (* TODO: are these all needed? *)
+  Local Existing Instance rep.Z.
+  Local Instance sem_ok : Semantics.parameters_ok semantics
+    := semantics_ok.
+  Local Instance mem_ok : map.ok Semantics.mem
+    := Semantics.mem_ok.
+  Local Instance varname_eqb_spec x y : BoolSpec _ _ _
+    := Decidable.String.eqb_spec x y.
+
+  (* separation-logic relation that says space exists in memory for lists
+     (other values are ignored) *)
+  Fixpoint lists_reserved {t}
+    : base_list_lengths t ->
+      Semantics.mem -> (* memory *)
+      Prop :=
+    match t with
+    | base.type.prod a b =>
+      fun x => sep (lists_reserved (fst x)) (lists_reserved (snd x))
+    | base_listZ =>
+      fun n =>
+        Lift1Prop.ex1
+          (fun start : Semantics.word =>
+             Lift1Prop.ex1
+               (fun oldvalues : list Semantics.word =>
+                  let size := Interface.word.of_Z (Z.of_nat n) in
+                  array scalar size start oldvalues))
+    | base_Z => fun _ _ => True
+    |  _ => fun _ _ => False
+    end.
+
+  Fixpoint list_lengths_from_value {t}
+    : base.interp t -> base_list_lengths t :=
+    match t as t0 return base.interp t0 -> base_list_lengths t0 with
+    | base.type.prod a b =>
+      fun x : base.interp a * base.interp b =>
+        (list_lengths_from_value (fst x),
+         list_lengths_from_value (snd x))
+    | base_listZ => fun x : list Z => length x
+    | _ => fun _ => tt
+    end.
+
+  Fixpoint list_lengths_from_args {t}
+    : type.for_each_lhs_of_arrow API.interp_type t ->
+      type.for_each_lhs_of_arrow list_lengths t :=
+    match t with
+    | type.base b => fun _ => tt
+    | type.arrow (type.base a) b =>
+      fun x =>
+        (list_lengths_from_value (fst x), list_lengths_from_args (snd x))
+    | type.arrow a b =>
+      fun x => (tt, list_lengths_from_args (snd x))
+    end.
+
+  (* TODO : remove
+
+  Definition load_list (start : Syntax.expr.expr) (len nextn : nat)
+    : nat * list string * Syntax.cmd.cmd :=
+    let exprs := map (load_list_item start) (seq 0 len) in
+    let varnames := map varname_gen (seq nextn len) in
+    let sets := map2 cmd.set varnames exprs in
+    (len, varnames, fold_right cmd.seq cmd.skip sets). *)
+  Eval simpl in
+ ( Language.Compilers.base.interp Compilers.base_interp
+                                  base_listZ).
+  Eval cbn in (fun mem (x : base_ltype (listZ:=rep.listZ_mem) base_listZ) (y : _) =>
+                   WeakestPrecondition.dexprs mem map.empty (flatten_base_rtype (base_rtype_of_ltype x)) [y]).
+  Print WeakestPrecondition.dexprs.
+  About WeakestPrecondition.expr.
+  Print rep.listZ_mem.
+  Print rep.equiv.
+  Lemma load_list_correct :
+    forall (len nextn : nat)
+           (name : base_ltype (listZ:=rep.listZ_mem) base_listZ)
+           (start : Semantics.word)
+           (l : list Z)
+           (tr : Semantics.trace)
+           (locals : Semantics.locals)
+           (mem : Semantics.mem)
+           (functions : list _)
+           (R : Semantics.mem -> Prop),
+      (forall (n : nat) (H : nextn <= n), name <> varname_gen n) ->
+      sep (rep.equiv (t:=base_listZ) l (base_rtype_of_ltype name) locals) R mem ->
+      WeakestPrecondition.expr
+        mem map.empty (expr.var name) (eq start) ->
+      (* load_list returns # vars used, variable names, cmd *)
+      let out := load_list (expr.var name) len nextn in
+      let nvars := fst (fst out) in
+      let names' : base_ltype (listZ:=rep.listZ_local) base_listZ
+          := snd (fst out) in
+      WeakestPrecondition.cmd
+        (WeakestPrecondition.call functions)
+        (snd out)
+        tr mem locals
+        (fun tr' mem' locals' =>
+           tr = tr' /\
+           mem = mem' /\
+           Interface.map.only_differ
+             locals (used_varnames nextn nvars) locals' /\
+           (forall n,
+               (nextn + nvars <= n)%nat ->
+               ~ varname_set names' (varname_gen n)) /\
+           locally_equivalent (t:=base_listZ)
+                              l (base_rtype_of_ltype names') locals').
+  Admitted.
+
+  Lemma load_all_lists_correct {t} :
+    forall (argnames : base_ltype t)
+           (args : base.interp t)
+           (flat_args : list Semantics.word)
+           (functions : list _)
+           (tr : Semantics.trace)
+           (locals : Semantics.locals)
+           (mem : Semantics.mem)
+           (nextn : nat)
+           (R : Semantics.mem -> Prop),
+        (* lengths of any lists in the arguments *)
+        let arglengths := list_lengths_from_value args in
+        (* look up variables in argnames *)
+        let argvalues := base_rtype_of_ltype argnames in
+        (* argnames don't contain variables we could later overwrite *)
+        (forall n,
+            (nextn <= n)%nat ->
+            ~ varname_set argnames (varname_gen n)) ->
+        (* argument values (in their 3 forms) are equivalent *)
+        sep (equivalent args argvalues locals) R mem ->
+        WeakestPrecondition.dexprs
+          mem map.empty (flatten_base_rtype argvalues) flat_args ->
+        (* load_all_lists returns triple : # fresh variables used,
+           new argnames with local lists, and cmd *)
+        let out := load_all_lists nextn argnames arglengths in
+        let nvars := fst (fst out) in
+        (* extract loaded argument values *)
+        let argnames' := snd (fst out) in
+        let argvalues' := base_rtype_of_ltype argnames' in
+        (* translated function produces equivalent results *)
+        WeakestPrecondition.cmd
+          (WeakestPrecondition.call functions)
+          (snd out)
+          tr mem locals
+          (fun tr' mem' locals' =>
+             tr = tr' /\
+             mem = mem' /\
+             Interface.map.only_differ
+               locals (used_varnames nextn nvars) locals' /\
+             (forall n,
+                 (nextn + nvars <= n)%nat ->
+                 ~ varname_set argnames' (varname_gen n)) /\
+             locally_equivalent args argvalues' locals').
+  Proof.
+    induction t;
+      cbn [fst snd load_all_lists varname_set
+               locally_equivalent equivalent rep.equiv
+               rep.varname_set rep.Z
+          ]; break_match; intros;
+        repeat match goal with
+                 | _ => progress cleanup
+                 | H : sep (emp _) _ _ |- _ =>
+                   apply sep_emp_l in H
+                 | H : sep (fun _ => False) _ _ |- _ =>
+                   exfalso; cbv [sep] in H; cleanup; tauto
+               end.
+    { (* base_Z *)
+      straightline.
+      repeat match goal with
+               |- _ /\ _ => split end;
+        cbv [emp]; eauto using only_differ_zero with lia. }
+    { (* product *)
+      straightline.
+      eapply Proper_cmd; [ solve [apply Proper_call] | | ].
+      2:{ eapply IHt1; eauto.
+          { intros.
+            match goal with
+            | H : _ |- _ =>
+              setoid_rewrite not_union_iff in H;
+                apply H; eauto
+            end. }
+          { cbn [base_rtype_of_ltype fst snd] in *.
+            match goal with
+              H : sep _ _ _ |- _ =>
+              simple refine (Lift1Prop.subrelation_iff1_impl1 _ _ _ _ _ H)
+            end.
+            ecancel. }
+          { cbn [flatten_base_rtype base_rtype_of_ltype fst snd] in *.
+            match goal with
+              H : WeakestPrecondition.dexprs _ _ (_ ++ _) _ |- _ =>
+              apply dexprs_app_l in H; cleanup
+            end.
+            eassumption. } }
+      repeat intro. cleanup; subst.
+      eapply Proper_cmd; [ solve [apply Proper_call] | | ].
+      2:{ eapply IHt2; eauto.
+          { intros.
+            match goal with
+            | H : _ |- _ =>
+              setoid_rewrite not_union_iff in H;
+                apply H; lia
+            end. }
+          { cbn [base_rtype_of_ltype fst snd] in *.
+            eapply Proper_sep_iff1; [ | reflexivity | ].
+            { eapply equivalent_only_differ_iff1;
+                eauto using equiv_listZ_only_differ_mem, only_differ_sym.
+              intros.
+              match goal with H : _ |- _ =>
+                              rewrite used_varnames_iff in H end.
+              cleanup. subst.
+              match goal with
+              | H : _ |- _ =>
+                setoid_rewrite not_union_iff in H;
+                  apply H; eauto
+              end. }
+            match goal with
+              H : sep _ _ _ |- _ =>
+              simple refine (Lift1Prop.subrelation_iff1_impl1 _ _ _ _ _ H)
+            end.
+            ecancel. }
+          { cbn [flatten_base_rtype base_rtype_of_ltype fst snd] in *.
+            match goal with
+              H : WeakestPrecondition.dexprs _ _ (_ ++ _) _ |- _ =>
+              apply dexprs_app_l in H; cleanup
+            end.
+            eassumption. } }
+      cbn [list_lengths_from_value fst snd] in *.
+      repeat intro. cleanup; subst.
+      repeat match goal with |- _ /\ _ => split end;
+        eauto using only_differ_step.
+      { intros; apply not_union_iff; split;
+          match goal with H : _ |- _ => apply H; lia end. }
+      { cbv [locally_equivalent locally_equivalent_args] in *.
+        cbn [equivalent_args fst rtype_of_ltype].
+        apply sep_empty_iff; split; eauto.
+        eapply equivalent_only_differ_iff1;
+          eauto using equiv_listZ_only_differ_local, only_differ_sym.
+        intros.
+        match goal with H : _ |- _ =>
+                        rewrite used_varnames_iff in H end.
+        cleanup. subst.
+        match goal with H : _ |- _ => apply H; lia end. } }
+  { (* base_listZ *)
+     clear IHt.
+
+    }
+  Qed.
+
+  Lemma load_arguments_correct {t} :
+    forall (argnames : type.for_each_lhs_of_arrow ltype t)
+           (args : type.for_each_lhs_of_arrow API.interp_type t)
+           (flat_args : list Semantics.word)
+           (functions : list _)
+           (tr : Semantics.trace)
+           (locals : Semantics.locals)
+           (mem : Semantics.mem)
+           (nextn : nat)
+           (R : Semantics.mem -> Prop),
+        (* lengths of any lists in the arguments *)
+        let arglengths := list_lengths_from_args args in
+        (* look up variables in argnames *)
+        let argvalues :=
+            type.map_for_each_lhs_of_arrow rtype_of_ltype argnames in
+        (* argnames don't contain variables we could later overwrite *)
+        (forall n,
+            (nextn <= n)%nat ->
+            ~ varname_set_args argnames (varname_gen n)) ->
+        (* argument values (in their 3 forms) are equivalent *)
+        sep (equivalent_args args argvalues locals) R mem ->
+        WeakestPrecondition.dexprs
+          mem map.empty (flatten_args argvalues) flat_args ->
+        (* load_arguments returns triple : # fresh variables used,
+           new argnames with local lists, and cmd *)
+        let out := load_arguments nextn argnames arglengths in
+        let nvars := fst (fst out) in
+        (* extract loaded argument values *)
+        let argnames' := snd (fst out) in
+        let argvalues' :=
+            type.map_for_each_lhs_of_arrow rtype_of_ltype argnames' in
+        (* translated function produces equivalent results *)
+        WeakestPrecondition.cmd
+          (WeakestPrecondition.call functions)
+          (snd out)
+          tr mem locals
+          (fun tr' mem' locals' =>
+             tr = tr' /\
+             mem = mem' /\
+             Interface.map.only_differ
+               locals (used_varnames nextn nvars) locals' /\
+             (forall n,
+                 (nextn + nvars <= n)%nat ->
+                 ~ varname_set_args argnames' (varname_gen n)) /\
+             locally_equivalent_args args argvalues' locals').
+  Proof.
+    cbv zeta.
+    induction t;
+      destruct argnames;
+      cbn [fst snd load_arguments
+               list_lengths_from_args varname_set_args
+               type.for_each_lhs_of_arrow equivalent_args
+               type.map_for_each_lhs_of_arrow flatten_args
+               ]; break_match; intros.
+    { (* base type *)
+      straightline.
+      repeat match goal with
+             | |- _ /\ _ => split end;
+        eauto using only_differ_zero; try reflexivity. }
+    { (* arrow (base _) _ *)
+      match goal with
+      | |- context [let '(x, y) := ?z in _] =>
+        rewrite (surjective_pairing z); cbn [fst snd] in *
+      end.
+      match goal with
+      | H : _ |- _ => apply dexprs_app_l in H
+      end.
+      cleanup.
+      straightline.
+      eapply Proper_cmd.
+      3:{
+        eapply load_all_lists_correct.
+        { intros.
+          match goal with
+            | H : _ |- _ =>
+          setoid_rewrite not_union_iff in H;
+            apply H; eauto
+          end. }
+        { match goal with
+          | H : sep (sep ?p ?q) ?r ?m |-
+            sep ?p _ ?m =>
+            apply sep_assoc in H; apply H
+          end. }
+        { eauto. } }
+      { apply Proper_call. }
+      { repeat intro; cleanup; subst.
+        eapply Proper_cmd; [ solve [apply Proper_call] | | ].
+        2:{
+          eapply IHt2; eauto.
+        { intros.
+          match goal with
+            | H : _ |- _ =>
+          setoid_rewrite not_union_iff in H;
+            apply H; lia
+          end. }
+        {
+          match goal with
+          | H : sep (sep ?p ?q) ?r ?m |- sep _ _ ?m =>
+            apply sep_comm, sep_assoc, sep_comm in H;
+            eapply Proper_sep_iff1; [ | reflexivity | apply H]
+          end.
+          eapply equivalent_args_only_differ_iff1;
+            eauto using equiv_listZ_only_differ_mem, only_differ_sym.
+          intros.
+          match goal with H : _ |- _ =>
+                          rewrite used_varnames_iff in H end.
+          cleanup. subst.
+          match goal with
+            | H : _ |- _ =>
+          setoid_rewrite not_union_iff in H;
+            apply H; eauto
+          end. } }
+        { repeat intro. cleanup. subst.
+          repeat match goal with |- _ /\ _ => split end;
+            eauto using only_differ_step.
+          { intros; apply not_union_iff; split;
+              match goal with H : _ |- _ => apply H; lia end. }
+          { cbv [locally_equivalent locally_equivalent_args] in *.
+            cbn [equivalent_args fst rtype_of_ltype].
+            apply sep_empty_iff; split; eauto.
+            eapply equivalent_only_differ_iff1;
+              eauto using equiv_listZ_only_differ_local, only_differ_sym.
+            intros.
+            match goal with H : _ |- _ =>
+                            rewrite used_varnames_iff in H end.
+            cleanup. subst.
+            eauto with lia. } } } }
+    { (* arrow (arrow _ _) _ *)
+      match goal with
+      | H : sep (fun _ => False) _ _ |- _ =>
+        exfalso; cbv [sep] in H; cleanup; tauto
+      end. }
+  Qed.
+
+  (* idea: pull return list lengths from fiat-crypto type *)
+  Lemma store_return_values_correct {t} :
+    forall (retnames_local : base_ltype t)
+           (retnames_mem : base_ltype t)
+           (retlengths : base_list_lengths t)
+           (rets : base.interp t)
+           (functions : list _)
+           (tr : Semantics.trace)
+           (locals : Semantics.locals)
+           (mem : Semantics.mem)
+           (R : Semantics.mem -> Prop),
+        (* use old values of memory to set up frame for return values *)
+        sep (lists_reserved retlengths) R mem ->
+        (* rets are stored in local retnames *)
+        locally_equivalent
+          rets (base_rtype_of_ltype retnames_local) locals ->
+        (* translated function produces equivalent results *)
+        WeakestPrecondition.cmd
+          (WeakestPrecondition.call functions)
+          (store_return_values retnames_local retnames_mem)
+          tr mem locals
+          (fun tr' mem' locals' =>
+             tr = tr' /\
+             sep (equivalent
+                    rets (base_rtype_of_ltype retnames_mem) locals')
+                 R mem').
+  Proof.
+  Admitted.
+End LoadStoreList.
